\documentclass[a4paper,12pt]{article}
%%%%%%%%%%%%%%%%%%%%%%%%%%%%%%%%%%%%%%%%%%%%%%%%%%%%%%%%%%%%%%%%%%%%%%%%%%%%%%%%%%%%%%%%%%%%%%%%%%%%%%%%%%%%%%%%%%%%%%%%%%%%%%%%%%%%%%%%%%%%%%%%%%%%%%%%%%%%%%%%%%%%%%%%%%%%%%%%%%%%%%%%%%%%%%%%%%%%%%%%%%%%%%%%%%%%%%%%%%%%%%%%%%%%%%%%%%%%%%%%%%%%%%%%%%%%
\usepackage{eurosym}
\usepackage{vmargin}
\usepackage{amsmath}
\usepackage{graphics}
\usepackage{epsfig}
\usepackage{enumerate}
\usepackage{multicol}
\usepackage{subfigure}
\usepackage{fancyhdr}
\usepackage{listings}
\usepackage{framed}
\usepackage{graphicx}
\usepackage{amsmath}
\usepackage{chngpage}
%\usepackage{bigints}

\usepackage{vmargin}
% left top textwidth textheight headheight
% headsep footheight footskip
\setmargins{2.0cm}{2.5cm}{16 cm}{22cm}{0.5cm}{0cm}{1cm}{1cm}
\renewcommand{\baselinestretch}{1.3}

\setcounter{MaxMatrixCols}{10}

\begin{document}

\begin{enumerate}
\item The distribution is defined in the area shown by the shaded triangle.

\item  fx(x) =
R a¡x
0 f(x; y)dy = 2
a2
R a¡x
0 dy = 2(a¡x)
a2 for 0 · x · a; and 0 otherwise
FX(x) =
R x
0 fX(u)du = 2
a2
R x
0 (a ¡ u)du = 2
a2 [au ¡ 1
2u2]x
0 = 2ax¡x2
a2 for 0 · x · a.
4
\item E[X] =
R a
0 xfX(x)dx = 2
a2
R a
0 x(a ¡ x)dx = 2
a2 [ 1
2ax2 ¡ 1
3x3]a
0 = a
3 by symmetry,E[Y ] = a
3
also.
\item 

\begin{eqnarray*}
E(X) &=& \int^{a}_{0} x \;f_X(x) dx \\
    &=&\int^{a}_{0} x(a-x) dx \\
    &=&  \frac{2}{a^2}\left[ \frac{1}{2}ax^2 - \frac{1}{3}x^3  \right]^{a}_{0}\\
    &=& \frac{a}{3}  
\end{eqnarray*}
Similarly $E(Y) = \frac{a}{3} $

\begin{eqnarray*}
E(X^2) &=& \int^{a}_{0} x^2 \;f_X(x) dx \\
    &=&\int^{a}_{0} x^2(a-x) dx \\
    &=&  \frac{2}{a^2}\left[ \frac{1}{3}ax^3 - \frac{1}{4}x^4  \right]^{a}_{0}\\
    &=& \frac{a^2}{6}  
\end{eqnarray*}
Similarly $E(Y^2) = \frac{a^2}{6} $

\begin{eqnarry*}
Var(X) &=& [E(X^2)] - [E(X)^2] \\
      &=& \frac{a^2}{6} - \left(\frac{a}{3}\right)^2 \\
     &=& \frac{a^2}{18} \\
\end{eqnarray*}
Necessarily $Var(X) = \frac{a^2}{18}$


\item  E[XY ] =
R a
x=0
R a=x
y=0 xyf(x; y)dydx =
R a
0 xf
R a¡x
0
2y
a2 dygdx
=
R a
0 x[ y2
a2 ]a¡x
0 dx = 1
a2
R a
0 x(a ¡ x)2dx = 1
a2
R a
0 (a2x ¡ 2ax2 + x3)dx
= 1
a2 [ 1
2a2x2 ¡ 2
3ax3 + 1
4x4]a
0 = 1
12a2.
Cov(X; Y ) = E[XY ] ¡ E[X]E[Y ] = a2
12 ¡ fraca32 = a2( 1
12 ¡ 1
9 = ¡a2
36 ,
Hence Pxy = pcov(X;Y )
V (X)V (Y )
= ¡a2=36
a2=18 = ¡1=2:
\end{enumerate}
\end{document}
