\documentclass[a4paper,12pt]{article}
%%%%%%%%%%%%%%%%%%%%%%%%%%%%%%%%%%%%%%%%%%%%%%%%%%%%%%%%%%%%%%%%%%%%%%%%%%%%%%%%%%%%%%%%%%%%%%%%%%%%%%%%%%%%%%%%%%%%%%%%%%%%%%%%%%%%%%%%%%%%%%%%%%%%%%%%%%%%%%%%%%%%%%%%%%%%%%%%%%%%%%%%%%%%%%%%%%%%%%%%%%%%%%%%%%%%%%%%%%%%%%%%%%%%%%%%%%%%%%%%%%%%%%%%%%%%
\usepackage{eurosym}
\usepackage{vmargin}
\usepackage{amsmath}
\usepackage{graphics}
\usepackage{epsfig}
\usepackage{enumerate}
\usepackage{multicol}
\usepackage{subfigure}
\usepackage{fancyhdr}
\usepackage{listings}
\usepackage{framed}
\usepackage{graphicx}
\usepackage{amsmath}
\usepackage{chngpage}
%\usepackage{bigints}

\usepackage{vmargin}
% left top textwidth textheight headheight
% headsep footheight footskip
\setmargins{2.0cm}{2.5cm}{16 cm}{22cm}{0.5cm}{0cm}{1cm}{1cm}
\renewcommand{\baselinestretch}{1.3}

\setcounter{MaxMatrixCols}{10}

\begin{document}
\begin{enumerate}
    \item  For u = 1/2; 
    
\begin{itemize}   
\item P(0) = e-1=2 = 0:60653; 
\item P(1) = 0:30327; 
\item P(2) = 0:07582
\item P(3) =
0:01264
\item P(¸ 4)very small.
\end{itemize}

For u = 2; 
\begin{itemize}   
\item p(0) = 0:13534; 
\item p(1) = 0:27067 
\item p(2); 
\item p(3) = 0:18045; 
\item p(5) = 0:03609; 
\item p(6) = 0:01203
\end{itemize}
%%%%%%%%%%%%%%%%%%%%%%%%%%%%%%%%%%%%%%%%%%%
\item  (a) The sampling method does not collect any data for which y=0. Hence in this distribution
1P
y=1
P(y) = 1
%------------------%
\begin{itemize}
\item But since we have a Poisson distribution originally we know that $P(y = 0) =
e^{-u}$;and $P(y ¸ 1) = 1 - e^{-u}$:
\item This the total probability for the data that have been collected is $1-e^{-u}$, and each
individual probability must be expressed as a proportion of this in order to make
them add to 1.
\item 
Therefore \[P(Y = y) = e^{-u}uy\]
\end{itemize}
%------------------%

$(1-e^{-u})y! for y = 1; 2; 3; \ldots$


\begin{eqnarray*}
E[Y] &=& 
\sum^{\infty}_{y=1} \frac{u^{y} \times y \times e^{-y} }{1-e^{-u}y!}\\
&=& \frac{u\times e^{-u}}{1-e^{-u}} \sum^{\infty}_{y=1} \frac{u^{y-1} }{(y-1)!}\\
&=& \frac{u \times e^{-u}}{1-e^{-u}} \sum^{\infty}_{y=1} \frac{u^{s} }{s!}\\
&=& \frac{u}{1-e^{-u}}
\end{eqnarray*}

 since the
P
s factor
equals eu.
\begin{itemize}
\item $E[Y ] - P(Y = 1) = u$
$1-e^{-u} - ue^{-u}$
$1-e^{-u} = u$
\item Hence the sample fraction of leaves with just one insect, subtract from the sample
mean (which is an unbiased estimate of $E[Y]$) gives an unbiased estimate of $u$.
\end{itemize}
\end{enumerate}
\end{document}
