\documentclass[a4paper,12pt]{article}
%%%%%%%%%%%%%%%%%%%%%%%%%%%%%%%%%%%%%%%%%%%%%%%%%%%%%%%%%%%%%%%%%%%%%%%%%%%%%%%%%%%%%%%%%%%%%%%%%%%%%%%%%%%%%%%%%%%%%%%%%%%%%%%%%%%%%%%%%%%%%%%%%%%%%%%%%%%%%%%%%%%%%%%%%%%%%%%%%%%%%%%%%%%%%%%%%%%%%%%%%%%%%%%%%%%%%%%%%%%%%%%%%%%%%%%%%%%%%%%%%%%%%%%%%%%%
\usepackage{eurosym}
\usepackage{vmargin}
\usepackage{amsmath}
\usepackage{graphics}
\usepackage{epsfig}
\usepackage{enumerate}
\usepackage{multicol}
\usepackage{subfigure}
\usepackage{fancyhdr}
\usepackage{listings}
\usepackage{framed}
\usepackage{graphicx}
\usepackage{amsmath}
\usepackage{chngpage}
%\usepackage{bigints}

\usepackage{vmargin}
% left top textwidth textheight headheight
% headsep footheight footskip
\setmargins{2.0cm}{2.5cm}{16 cm}{22cm}{0.5cm}{0cm}{1cm}{1cm}
\renewcommand{\baselinestretch}{1.3}

\setcounter{MaxMatrixCols}{10}
\begin{document}

% Higher Certificate, Paper I, 2001. Question 1



\begin{itemize}
\item[(a)] A and B are independent. So $P(A\cap B) = P(A)P(B)$ .
( ) 1 ( ) 1 ; ( ) 1 ; so ( ) 1
3 2 6
\begin{itemize}
    \item $P A = − P A = $
    \item $P B = $
    \item $P A\cap B = .$
\end{itemize}
\end{itemize}
%%%%%%%%%%%%%%%%%%%%


\begin{itemize}
\item[(b)] \[A\cap B = [(A\cap B)\cap C]\cup[(A\cap B)\cap C],\]
with the two events $[(A\cap B)\cap C]$ and $[(A\cap B)\cap C]$ being disjoint .
Hence ( ) ( ) ( ) 1 1 1
6 10 15
\[P A\cap B \cap C = P A\cap B − P A\cap B \cap C = − = .\]
\item  \[B\cap C = (A\cap B\cap C)\cup(A\cap B\cap C) \], these being disjoint.
\begin{itemize}
    \item Further, \[(A\cap B \cap C)\cup(A\cap B \cap C) = (A\cap B) .\]
\item Hence \[P(B \cap C) = P(A\cap B \cap C) + P(\bar{A} \cap B) − P(\bar{A} \cap \bar{B} \cap \bar{C})\]
\[P(B \cap C) =  \frac{1}{4}+ \left( \frac{1}{3} \times \frac{1}{2} \right) ×
 − P A\cap C − P A\cap B \cap C   \]
since A,B are independent.
\end{itemize}





\item But A, C are also independent and so are A,C .
\end{itemize}

Therefore ( ) 1 1 1 2 1 5 1 63
4 6 3 5 15 12 15 12 15
\begin{eqnarray*}
P P( B \cap C)  &=& \frac{1}{4} +\frac{1}{6} -\left( \frac{1}{3} \times \frac{2}{5} \right) + \frac{1}{15} \\
 &=& \frac{3}{12} +\frac{2}{12} -\left(  \frac{2}{15} \right) + \frac{1}{15}
 \\
 &=& \frac{5}{12} -\frac{1}{15}\\
 &=& \frac{25}{60} -\frac{4}{60}\\
  &=& \frac{21}{60} = \frac{7}{20}\\
\end{eqnarray*}

\item Compute $P (B | C)$

\[
P (B | C) = \frac{P( B \cap C)}{P (C)} = \frac{7/20}{3/5} = \frac{7/20}{12/20} = \frac{7}{12}\]

\item Compute $P (A | B  \cap C)$ 
\[
P (A | B  \cap C) = \frac{P( A \cap B \cap C)}{P (B \cap C)} = \frac{1/4}{7/20} = \frac{20}{28} = \frac{5}{7}\]

\item Compute $P (A \cap B | A \cap C)$ 
\[
P (A \cap B | A \cap C) = \frac{P( A \cap B \cap C)}{P (A \cap C)} = \frac{1/4}{2/3 \times 3/5} = \frac{1/4}{6/15} = \frac{15}{24} = \frac{5}{8}\]
(A, C are independent).
\end{enumerate}
\end{document}
