\documentclass[a4paper,12pt]{article}
%%%%%%%%%%%%%%%%%%%%%%%%%%%%%%%%%%%%%%%%%%%%%%%%%%%%%%%%%%%%%%%%%%%%%%%%%%%%%%%%%%%%%%%%%%%%%%%%%%%%%%%%%%%%%%%%%%%%%%%%%%%%%%%%%%%%%%%%%%%%%%%%%%%%%%%%%%%%%%%%%%%%%%%%%%%%%%%%%%%%%%%%%%%%%%%%%%%%%%%%%%%%%%%%%%%%%%%%%%%%%%%%%%%%%%%%%%%%%%%%%%%%%%%%%%%%
\usepackage{eurosym}
\usepackage{vmargin}
\usepackage{amsmath}
\usepackage{graphics}
\usepackage{epsfig}
\usepackage{enumerate}
\usepackage{multicol}
\usepackage{subfigure}
\usepackage{fancyhdr}
\usepackage{listings}
\usepackage{framed}
\usepackage{graphicx}
\usepackage{amsmath}
\usepackage{chngpage}
%\usepackage{bigints}

\usepackage{vmargin}
% left top textwidth textheight headheight
% headsep footheight footskip
\setmargins{2.0cm}{2.5cm}{16 cm}{22cm}{0.5cm}{0cm}{1cm}{1cm}
\renewcommand{\baselinestretch}{1.3}

\setcounter{MaxMatrixCols}{10}
\begin{document}\begin{table}[ht!]
     \centering
     \begin{tabular}{|p{15cm}|}
     \hline        
4. Two players, A and B, each simultaneously and independently roll a fair die.  Let X and Y be random variables denoting the respective scores of A and B on any given roll, so that 


\[   P(X=x,Y=y) = \begin{cases}  \frac{1}{6} & x,y= 1,2,3,4,5,6 \\
0 & \mbox{otherwise} \end{cases}\]

 
 
 
(i) Show that 
\[P(X=Y) = \frac{1}{6}\]
 
 
and that 
 
\[P(X>Y) = \frac{5}{12}\]
 
 \\ \hline
      \end{tabular}
    \end{table}

\begin{enumerate}
    \item 
    
\begin{eqnarray*}
P(x = y) &=& P(x = y = 1) + P(x = y = 2) + \ldots + P(x = y = 6)\\ 
&=& \frac{6}{36}\\
&=& \frac{1}{6}\\
\end{eqnarray*}

\begin{itemize}
    \item $P(x > y or y > x) = 1 - P(x = y) = 5$
\item By symmetry of the joint distribution,$P(x > y) = P(y > x)$, so each of these must be $ \frac{5}{12}$
\item ALTERNATIVELY enumerate all possibilities
\end{itemize}

\item 
\begin{eqnarray*}
P(z > k) &=& P(\mbox{neither A or B throws a 6 in first k - 1 attempts})\\
&=& (\frac{5}{6} \times \frac{5}{6} )k-1 \\
&=& (\frac{25}{36} )k-1; k = 1, 2, 3, \ldots
\end{eqnarray*}

\begin{eqnarray*}
P(z = k) &=& P(z \geq k) - P(z \geq k + 1)\\
&=& ( \frac{25}{36} )k-1(1 -  \left( \frac{25}{36} \right) \\
&=& ( \frac{11}{36} )( \frac{25}{36} )k-1 k = 1; 2; 3; \ldots
\end{eqnarray*}
%%%%%%%%%%%%%%%%%%%%%%%%%%%%%%%%%%%%%%%%%%%%%%%%%%%%%%5

    
  \begin{table}[ht!]
     \centering
     \begin{tabular}{|p{15cm}|}
     \hline  
(ii) Let Z be a random variable denoting the number of times A and B each have to roll their dice for one or both to score a six.  Explain why 
 
\[   P(Z=z) = \begin{cases}  \frac{11}{36} \left( \frac{25}{36} \right)^{z-1} & z= 1,2,3,ldots \\
0 & \mbox{otherwise} \end{cases}\]

 
 \\ \hline 
      \end{tabular}
    \end{table}
    
    
     

    
    
\item 
\begin{eqnarray*}
P(z \leq 4) &=& 1 - P(z \geq 5) \\
&=& 1 - \left( \frac{25}{36} \right)^4 \\
&=&  0.233
\end{eqnarray*}


\begin{eqnarray*}
E[z] &=&
1X
k=1
kP(z = k) \\ &=& \frac{11}{36} \times \sum^{\infty}_{\gamma=1} \gamma x 
\left(\frac{25}{36}
\right)^{\gamma-1}
\end{eqnarray*}
  \begin{table}[ht!]
     \centering
     \begin{tabular}{|p{15cm}|}
     \hline  
(iii) Making use of this result, find 
 
(a) $P(Z \leq 4)$ , (b) $E(Z)$ , 
 
giving your answers to 3 significant figures. 
 \\ \hline 
      \end{tabular}
    \end{table}
Now
$\sum^{\infty}_{\gamma=1} \gamma x ^{\gamma-1}$ is derivative of
1P
k=1
xk = 1
1-x by the used results for a geometric series.
Thus
\[\sum^{\infty}_{\gamma=1} \gamma x ^{\gamma-1} = d
dx ( 1
1-x ) = 1
(1-x)2 \], we have x = 25
36 ;
Therefore
\begin{eqnarray*}
E[z] &=& \frac{11}{36} \times \frac{1}{(1- \frac{25}{36})^2} \\ &=& \frac{36}{11} 
\\ &=& 3.27
\end{eqnarray*}
Alternatively consider E[z] and -25
36E[z], and add to give 11
36E[z] which is 1 as an
infinite geometric series
\end{enumerate}
\end{document}
